# Solutions to the 71st William Lowell Putnam Mathematical Competition

## Saturday, December 4, 2010

Kiran Kedlaya and Lenny Ng

A-1 The largest such  $k$  is  $\lfloor \frac{n+1}{2} \rfloor = \lceil \frac{n}{2} \rceil$ . For  $n$  even, this value is achieved by the partition

$$\{1, n\}, \{2, n-1\}, \dots;$$

for  $n$  odd, it is achieved by the partition

$$\{n\}, \{1, n-1\}, \{2, n-2\}, \dots.$$

One way to see that this is optimal is to note that the common sum can never be less than  $n$ , since  $n$  itself belongs to one of the boxes. This implies that  $k \le (1 + \dots + n)/n = (n+1)/2$ . Another argument is that if  $k > (n+1)/2$ , then there would have to be two boxes with one number each (by the pigeonhole principle), but such boxes could not have the same sum.

**Remark.** A much subtler question would be to find the smallest  $k$  (as a function of  $n$ ) for which no such arrangement exists.

A-2 The only such functions are those of the form  $f(x) = cx + d$  for some real numbers  $c, d$  (for which the property is obviously satisfied). To see this, suppose that  $f$  has the desired property. Then for any  $x \in \mathbb{R}$ ,

$$\begin{aligned} 2f'(x) &= f(x+2) - f(x) \\ &= (f(x+2) - f(x+1)) + (f(x+1) - f(x)) \\ &= f'(x+1) + f'(x). \end{aligned}$$

Consequently,  $f'(x+1) = f'(x)$ .

Define the function  $g: \mathbb{R} \to \mathbb{R}$  by  $g(x) = f(x+1) - f(x)$ , and put  $c = g(0)$ ,  $d = f(0)$ . For all  $x \in \mathbb{R}$ ,  $g'(x) = f'(x+1) - f'(x) = 0$ , so  $g(x) = c$  identically, and  $f'(x) = f(x+1) - f(x) = g(x) = c$ , so  $f(x) = cx + d$  identically as desired.

A-3 If  $a = b = 0$ , then the desired result holds trivially, so we assume that at least one of  $a, b$  is nonzero. Pick any point  $(a_0, b_0) \in \mathbb{R}^2$ , and let  $L$  be the line given by the parametric equation  $L(t) = (a_0, b_0) + (a, b)t$  for  $t \in \mathbb{R}$ . By the chain rule and the given equation, we have  $\frac{d}{dt}(h \circ L) = h \circ L$ . If we write  $f = h \circ L: \mathbb{R} \to \mathbb{R}$ , then  $f'(t) = f(t)$  for all  $t$ . It follows that  $f(t) = Ce^t$  for some constant  $C$ . Since  $|f(t)| \le M$  for all  $t$ , we must have  $C = 0$ . It follows that  $h(a_0, b_0) = 0$ ; since  $(a_0, b_0)$  was an arbitrary point,  $h$  is identically 0 over all of  $\mathbb{R}^2$ .

A-4 Put

$$N = 10^{10^{10^n}} + 10^{10^n} + 10^n - 1.$$

Write  $n = 2^m k$  with  $m$  a nonnegative integer and  $k$  a positive odd integer. For any nonnegative integer  $j$ ,

$$10^{2^m j} \equiv (-1)^j \pmod{10^{2^m} + 1}.$$

Since  $10^n \ge n \ge 2^m \ge m+1$ ,  $10^n$  is divisible by  $2^n$  and hence by  $2^{m+1}$ , and similarly  $10^{10^n}$  is divisible by  $2^{10^n}$  and hence by  $2^{m+1}$ . It follows that

$$N \equiv 1 + 1 + (-1) + (-1) \equiv 0 \pmod{10^{2^m} + 1}.$$

Since  $N \ge 10^{10^n} > 10^n + 1 \ge 10^{2^m} + 1$ , it follows that  $N$  is composite.

A-5 We start with three lemmas.

**Lemma 1.** If  $\mathbf{x}, \mathbf{y} \in G$  are nonzero orthogonal vectors, then  $\mathbf{x} * \mathbf{x}$  is parallel to  $\mathbf{y}$ .

*Proof.* Put  $\mathbf{z} = \mathbf{x} \times \mathbf{y} \ne 0$ , so that  $\mathbf{x}, \mathbf{y}$ , and  $\mathbf{z} = \mathbf{x} * \mathbf{y}$  are nonzero and mutually orthogonal. Then  $\mathbf{w} = \mathbf{x} \times \mathbf{z} \ne 0$ , so  $\mathbf{w} = \mathbf{x} * \mathbf{z}$  is nonzero and orthogonal to  $\mathbf{x}$  and  $\mathbf{z}$ . However, if  $(\mathbf{x} * \mathbf{x}) \times \mathbf{y} \ne 0$ , then  $\mathbf{w} = \mathbf{x} * (\mathbf{x} * \mathbf{y}) = (\mathbf{x} * \mathbf{x}) * \mathbf{y} = (\mathbf{x} * \mathbf{x}) \times \mathbf{y}$  is also orthogonal to  $\mathbf{y}$ , a contradiction.  $\square$ 

**Lemma 2.** If  $\mathbf{x} \in G$  is nonzero, and there exists  $\mathbf{y} \in G$  nonzero and orthogonal to  $\mathbf{x}$ , then  $\mathbf{x} * \mathbf{x} = 0$ .

*Proof.* Lemma 1 implies that  $\mathbf{x} * \mathbf{x}$  is parallel to both  $\mathbf{y}$  and  $\mathbf{x} \times \mathbf{y}$ , so it must be zero.  $\square$ 

**Lemma 3.** If  $\mathbf{x}, \mathbf{y} \in G$  commute, then  $\mathbf{x} \times \mathbf{y} = 0$ .

*Proof.* If  $\mathbf{x} \times \mathbf{y} \ne 0$ , then  $\mathbf{y} \times \mathbf{x}$  is nonzero and distinct from  $\mathbf{x} \times \mathbf{y}$ . Consequently,  $\mathbf{x} * \mathbf{y} = \mathbf{x} \times \mathbf{y}$  and  $\mathbf{y} * \mathbf{x} = \mathbf{y} \times \mathbf{x} \ne \mathbf{x} * \mathbf{y}$ .  $\square$ 

We proceed now to the proof. Assume by way of contradiction that there exist  $\mathbf{a}, \mathbf{b} \in G$  with  $\mathbf{a} \times \mathbf{b} \ne 0$ . Put  $\mathbf{c} = \mathbf{a} \times \mathbf{b} = \mathbf{a} * \mathbf{b}$ , so that  $\mathbf{a}, \mathbf{b}, \mathbf{c}$  are nonzero and linearly independent. Let  $\mathbf{e}$  be the identity element of  $G$ . Since  $\mathbf{e}$  commutes with  $\mathbf{a}, \mathbf{b}, \mathbf{c}$ , by Lemma 3 we have  $\mathbf{e} \times \mathbf{a} = \mathbf{e} \times \mathbf{b} = \mathbf{e} \times \mathbf{c} = 0$ . Since  $\mathbf{a}, \mathbf{b}, \mathbf{c}$  span  $\mathbb{R}^3$ ,  $\mathbf{e} \times \mathbf{x} = 0$  for all  $\mathbf{x} \in \mathbb{R}^3$ , so  $\mathbf{e} = 0$ .

Since  $\mathbf{b}, \mathbf{c}$ , and  $\mathbf{b} \times \mathbf{c} = \mathbf{b} * \mathbf{c}$  are nonzero and mutually orthogonal, Lemma 2 implies

$$\mathbf{b} * \mathbf{b} = \mathbf{c} * \mathbf{c} = (\mathbf{b} * \mathbf{c}) * (\mathbf{b} * \mathbf{c}) = 0 = \mathbf{e}.$$

Hence  $\mathbf{b} * \mathbf{c} = \mathbf{c} * \mathbf{b}$ , contradicting Lemma 3 because  $\mathbf{b} \times \mathbf{c} \ne 0$ . The desired result follows.

A-6 **First solution.** Note that the hypotheses on  $f$  imply that  $f(x) > 0$  for all  $x \in [0, +\infty)$ , so the integrand is a continuous function of  $f$  and the integral makes sense. Rewrite the integral as

$$\int_0^\infty \left(1 - \frac{f(x+1)}{f(x)}\right) dx,$$