$$\begin{array}{r@{\hspace{1em}}r@{\hspace{1em}}r}x_1 & -2x_2 & +x_3 = 0 \\ & 2x_2 & -8x_3 = 8 \\ & -3x_2 & +13x_3 = -9\end{array} \quad \begin{bmatrix} 1 & -2 & 1 & 0 \\ 0 & 2 & -8 & 8 \\ 0 & -3 & 13 & -9 \end{bmatrix}$$

Changing the coefficient of  $x_2$  from 2 to 1.

- The purpose of this step is to simplify the calculation in the next steps.
- To do it, we multiply the 2<sup>nd</sup> equation by  $\frac{1}{2}$ .

$$\begin{array}{r@{\hspace{1em}}r@{\hspace{1em}}r}x_1 & -2x_2 & +x_3 = 0 \\ & x_2 & -4x_3 = 4 \\ & -3x_2 & +13x_3 = -9\end{array} \quad \begin{bmatrix} 1 & -2 & 1 & 0 \\ 0 & 1 & -4 & 4 \\ 0 & -3 & 13 & -9 \end{bmatrix}$$